Weidenbach_Book/IsaSAT/IsaSAT_Initialisation.thy
@@ -2113,7 +2113,7 @@ definition finalise_init_code :: \<open>opts \<Rightarrow> twl_st_wl_heur_init \
     RETURN (M', N', D', Q', W', ((ns, m, the fst_As, the lst_As, next_search), to_remove),
        clvls, cach, lbd, take 1(replicate 160 (Pos 0)), init_stats,
        (fema, sema, ccount, 0, (\<phi>, 0, replicate (length \<phi>) False, 0, replicate (length \<phi>) False, 10000, 1000, 1),
-           reluctant_init), vdom, [], lcount, opts, [], ivdom)
+           reluctant_init, False), vdom, [], lcount, opts, [], ivdom)
      })\<close>
 
 lemma isa_vmtf_init_nemptyD: \<open>((ak, al, am, an, bc), ao, bd)
